CodeGeneration.v
@@ -1,3 +1,6 @@
+(* A bunch of disorganized notes about models for Rust code *)
+
+
 Search "Total".
 
 
